Final

natexp_compiler.v
@@ -4,48 +4,51 @@
   Project 4
 
 ------------------------------------------------
-4 Proving an expression compiler correct
-Formalize both an interpreter and a compiler for a simple language of arith-
-metical expressions, and show that both give the same results. Compile the
-expressions to code for a simple stack machine. Use dependent types to make
-Rocq aware of the fact that the compiled code will never lead to a run time error.
+
+This file has four sections:
+   - Definitions
+   - Expression Evaluator
+   - Non dependent implementation of RPN   (1) 
+   - Dependent types implementation of RPN (2) 
+
+The functions relating to RPN will be annotated with the number to
+differentiate if they are dependent or non dependent
 
  *)
-
-
 Require Import Stdlib.Strings.String.
 Require Import Stdlib.Lists.List.
 
-
-(*
-Inductive definition:
+(* 
+-----------------------------
+        Definitions 
  *)
-
 Definition lit := nat. 
 Definition binop := (lit -> lit -> lit). 
 
-(*Partial map*)
 (*
-Definition env := string -> option lit.
-Definition empty : env := (fun _ => None).
-Definition update (f : env) (x : string) (l : lit) : env :=
-  (fun y => if String.eqb x y then Some l else f y).
+Partial map: Includes option in env chosen not to do this
+ as it adds extra complexity.
+This could be solved by a dependent type or a Map type
  *)
 
-(*Total map: Defaults to 0*)
+(* Total map with as defaults element 0*)
 Definition env := string -> lit.
 Definition empty : env := (fun _ => 0).
 Definition update (f : env) (x : string) (l : lit) : env :=
   (fun y => if String.eqb x y then l else f y).
 
+(* 
+-----------------------------
+        Expressions 
+ *)
+(* Definition of Exp *)
 Inductive Exp : Set :=
   | Elit : lit -> Exp
   | Evar : string -> Exp
   | Ebinop : binop -> Exp -> Exp -> Exp
 .
-(*
-Semantics for Exp
- *)
+
+(* Semantics for Exp *)
 Fixpoint eval (e:Exp) (f:env) {struct e} : lit :=
 match e with
 | Elit l      => l
@@ -53,53 +56,55 @@ match e with
 | Ebinop op e1 e2 => op (eval e1 f) (eval e2 f)
 end.
 
-(*
-Stackbased Implementation 
+(* 
+  -----------------------------
+  Non dependent type stackbased implementation (1)
  *)
- 
-Inductive RPN : Type :=
-  | RPNlit : lit -> RPN
-  | RPNvar : string -> RPN
-  | RPNbinop : binop -> RPN
+
+(* Defintion of Non dependent RPN *)
+Inductive RPN1 : Type :=
+  | RPN1lit : lit -> RPN1
+  | RPN1var : string -> RPN1
+  | RPN1bin : binop -> RPN1
 .
 
-Fixpoint exp_to_rpnlist (e:Exp) {struct e} : list RPN :=
+(* Non dependent RPN1 compiler *)
+Fixpoint compiler1 (e:Exp) {struct e} : list RPN1 :=
 match e with
-| Elit l => RPNlit l :: nil
-| Evar s => RPNvar s :: nil
-| Ebinop op e1 e2 => exp_to_rpnlist e1 ++ exp_to_rpnlist e2 ++ RPNbinop op :: nil
+| Elit l => RPN1lit l :: nil
+| Evar s => RPN1var s :: nil
+| Ebinop op e1 e2 => compiler1 e1 ++ compiler1 e2 ++ RPN1bin op :: nil
 end.
 
-Fixpoint rpn_eval (inp: list RPN) (stack: list lit) (f : env) {struct inp} : option lit :=
+(* Non dependent rpn evaluator *)
+Fixpoint rpn_eval1 (inp: list RPN1) (stack: list lit) (f : env) {struct inp} : option lit :=
 match inp with
 | nil => 
   match stack with
   | x::xs => Some x
   | nil  => None
   end
-| (RPNlit   l ) :: rs => rpn_eval rs (l  ::stack) f
-| (RPNvar   s ) :: rs => rpn_eval rs (f s::stack) f
-| (RPNbinop op) :: rs =>
+| (RPN1lit   l ) :: rs => rpn_eval1 rs (l  ::stack) f
+| (RPN1var   s ) :: rs => rpn_eval1 rs (f s::stack) f
+| (RPN1bin op) :: rs =>
   match stack with
-  | x::x'::xs => rpn_eval rs ((op x' x)::xs) f
+  | x::x'::xs => rpn_eval1 rs ((op x' x)::xs) f
   | _         => None
   end
 end.
 
-Definition rpn0:(list RPN) := (RPNlit 1) :: (RPNlit 2) :: (RPNbinop plus)::nil.
-Definition rpn1:(list RPN) := (RPNlit 3) :: (RPNlit 1) :: (RPNlit 2) :: (RPNbinop plus) :: (RPNbinop plus)::nil.
-Definition rpn2:(list RPN) := (RPNlit 3) :: (RPNlit 1) :: (RPNlit 2) :: (RPNbinop plus) :: (RPNbinop mult)::nil.
-Eval compute in (rpn_eval (rpn2) nil empty).
-Definition rpn3:(list RPN) := (RPNvar "x") :: (RPNlit 2) :: (RPNbinop plus)::nil.
-(*
-Eval compute in (rpn_eval (rpn3) nil env0).
-Eval compute in (rpn_eval (rpn3) nil empty).
- *)
+(* Some basic sanity checks *)
+Definition rpn0:(list RPN1) := (RPN1lit 1) :: (RPN1lit 2) :: (RPN1bin plus)::nil.
+Definition rpn1:(list RPN1) := (RPN1lit 3) :: (RPN1lit 1) :: (RPN1lit 2) :: (RPN1bin plus) :: (RPN1bin plus)::nil.
+Definition rpn2:(list RPN1) := (RPN1lit 3) :: (RPN1lit 1) :: (RPN1lit 2) :: (RPN1bin plus) :: (RPN1bin mult)::nil.
+Eval compute in (rpn_eval1 (rpn2) nil empty).
+Definition rpn3:(list RPN1) := (RPN1var "x") :: (RPN1lit 2) :: (RPN1bin plus)::nil.
 
-Lemma rpn_applied :
-  forall (e : Exp) (f : env) (st : list lit) (rpn : list RPN),
-    rpn_eval (exp_to_rpnlist e ++ rpn) st f =
-    rpn_eval rpn (eval e f :: st) f.
+(* Helper lemma which signifies one step of the rpn_eval1 while keeping the expression intact *)
+Lemma rpn_eval1_applied:
+  forall (e : Exp) (f : env) (st : list lit) (rpn : list RPN1),
+    rpn_eval1 (compiler1 e ++ rpn) st f =
+    rpn_eval1 rpn (eval e f :: st) f.
 Proof.
   (* We do not need to use a different environment in the induction step*)
   intros e f.
@@ -109,7 +114,7 @@ Proof.
   simpl; try reflexivity.
   (* Solve Binop case*)
   - intros st rpn.
-    (* Reshuffle list to get into a form of (exp_to_rpnlist e1 ++ (exp_to_rpnlist e2 ++ rpn)) *)
+    (* Reshuffle list to get into a form of (compiler1 e1 ++ (compiler1 e2 ++ rpn)) *)
     rewrite <- app_assoc. 
     rewrite <- app_assoc. 
     rewrite <- app_comm_cons. 
@@ -120,22 +125,23 @@ Proof.
     reflexivity.
 Qed.
 
-
 (*
 Prove that
 forall e:Exp, Some (eval e) = rpn_eval (rpn e)
+
+Aka: prove equivalence with non dependent types
  *)
-Lemma equivalent_under_extensionality : forall (f:env) (e:Exp), 
-  Some (eval e f) = rpn_eval (exp_to_rpnlist e) nil f.
+Lemma equivalent1 : forall (f:env) (e:Exp), 
+  Some (eval e f) = rpn_eval1 (compiler1 e) nil f.
 Proof.
   intros f e.
-  (* Delay the inductive step to the helper Lemma rpn_applied *)
+  (* Delay the inductive step to the helper Lemma rpn_eval1_applied *)
   destruct e; 
   (* Solve trivial cases (Lit and Var) *)
   simpl; try reflexivity.
   (* Solve Binop case by applying the rpn_eval twice *)
-  - rewrite rpn_applied.
-    rewrite rpn_applied.
+  - rewrite rpn_eval1_applied.
+    rewrite rpn_eval1_applied.
     reflexivity.
 Qed.
 
@@ -146,44 +152,53 @@ definition of rpn_eval, and explain how you need to modify your formal-
 ization in Rocq.
 
 ANSWER:
-   We could make the steps in the stack explicit. We would need a dependent type for stack which keeps track of the stack size after evaluation. This would be +1 for the Lit and Var case and -1 for the Binop case as we remove 2 stack elements and add one.
+   We could make the steps in the stack explicit. We would need a dependent type 
+   for the RPN list which keeps track of the stack size after evaluation. 
+   This would be +1 for the Lit and Var case and -1 for the Binop case as we 
+   remove 2 stack elements and add one. We encode this as S (S n) -> (S n) 
+   instead of (S n) -> n to ensure that the stack has enough Lits and/or 
+   Vars to evaluate a Binop.
+
+   Then we create a dependent structure that looks like a vector 
+
    When we return this dependent type with value 1 we know that when the program type checks it has a valid stack (where the evaluated length is 1).
-   As we do not have negative numbers in 'nat' we model the difference with two nats as follows:
+   As we do not have negative numbers in 'nat' we model the difference each instruction takes with two nats as follows:
  *)
-
-
-(* Does not compile as the execution needs a negative stack length *)
-(*
-Definition test1 := LScons (RPNlit' 1) (LScons (RPNlit' 2) (LScons (RPNbin' plus) LSnil)).
- *)
-(* Does not compile as the stack ends not equal to 1 *)
-(*
-Definition test2 : ListWithEvalSize 1 := LScons (RPNlit' 1) (LScons (RPNlit' 2) LSnil).
- *)
-
-(* I do not know how to get this working: 
-   - In each situation i tried we still need to match on a empty stack. This is not reachable because of the ListWithEvalSize 1 but i cannot connect the two.
-*)
 
 
 Require Import Coq.Vectors.Vector.
 (*Makes working with vectors less verbose *)
 Import VectorNotations.
 
-Inductive Instr : nat -> nat -> Type :=
-| I_lit {n} : lit -> Instr n (S n)
-| I_var {n} : string -> Instr n (S n)
-| I_bin {n} : binop -> Instr (S (S n)) (S n).
+(* The instructions with their stack difference *)
+Inductive RPN2 : nat -> nat -> Type :=
+| RPN2lit {n} : lit -> RPN2 n (S n)
+| RPN2var {n} : string -> RPN2 n (S n)
+| RPN2bin {n} : binop -> RPN2 (S (S n)) (S n).
 
-Inductive RPNdep : nat -> nat -> Type :=
-| R_nil  {n} : RPNdep n n
-| R_cons {n m k} : Instr n m -> RPNdep m k -> RPNdep n k.
+(* 
+   R_nil needs to be 1 here as we want the length of the evaluated RPNvec to be 1 
+*)
+Inductive RPNvec : nat -> Type :=
+| R_nil  : RPNvec 1 
+| R_cons {n m} : RPN2 n m -> RPNvec m -> RPNvec n.
 
-Fixpoint eval_instr {n m} (ins: Instr n m) (f : env) : Vector.t lit n -> Vector.t lit m :=
-match ins in Instr n' m' return Vector.t lit n' -> Vector.t lit m' with
-| I_lit l  => fun st => l::st
-| I_var s  => fun st => f s::st
-| I_bin op => fun st =>
+Fixpoint compiler2 {n} (e : Exp) : RPNvec (S n) -> RPNvec n :=
+match e with
+| Elit l          => fun c => R_cons (RPN2lit l) c
+| Evar s          => fun c => R_cons (RPN2var s) c
+| Ebinop op e1 e2 => fun c => compiler2 e1 (compiler2 e2 
+    (R_cons (RPN2bin op) c)) 
+end.
+
+Definition rpn := compiler2 (Ebinop plus (Elit 1) (Evar "a")) R_nil.
+Eval compute in rpn.
+
+Fixpoint eval_instr {n m} (ins: RPN2 n m) (f : env) : Vector.t lit n -> Vector.t lit m :=
+match ins with
+| RPN2lit l  => fun st => l::st
+| RPN2var s  => fun st => f s::st
+| RPN2bin op => fun st =>
   let x   := hd st in
   let st' := tl st in
   let y   := hd st' in
@@ -191,18 +206,66 @@ match ins in Instr n' m' return Vector.t lit n' -> Vector.t lit m' with
     op y x :: xs
 end.
 
-Fixpoint exec {n m} (c : RPNdep n m) (f : env)
-  : Vector.t lit n -> Vector.t lit m :=
-match c in RPNdep n' m' return Vector.t lit n' -> Vector.t lit m' with
+
+Fixpoint rpn_eval2 {n} (c : RPNvec n) (f : env)
+  : Vector.t lit n -> Vector.t lit 1 :=
+match c with
 | R_nil       => fun st => st
 | R_cons i c' => fun st =>
-    exec c' f (eval_instr i f st)
+    rpn_eval2 c' f (eval_instr i f st) 
 end.
 
-Fixpoint exp_to_rpndepvec {n k} (e : Exp) : RPNdep (S n) k -> RPNdep n k :=
-match e with
-| Elit l          => fun c => R_cons (I_lit l) c
-| Evar s          => fun c => R_cons (I_var s) c
-| Ebinop op e1 e2 => fun c => exp_to_rpndepvec e1 (exp_to_rpndepvec e2 (R_cons (I_bin op) c))
-end.
+(* 
+Some experimentation that the implementation is correct 
+ *)
+Definition test := rpn_eval2 rpn empty.
+Eval compute in test.
+Definition test' := rpn_eval2 rpn (update empty "a" 1).
+Eval compute in test'.
+Definition rpn'' := R_nil.
+(*Definition test'' := rpn_eval2 rpn'' empty.*)
+Definition rpn''' := R_cons (RPN2bin plus) R_nil.
+(*Definition test''' := rpn_eval2 rpn''' empty.*)
+(*Definition rpn'''' := R_cons (RPN2lit 1) (R_cons (RPN2lit 2) R_nil).*)
+(*Definition test'''' := rpn_eval2 rpn'''' empty.*)
+
+
+(* 
+The intermediate step (between IHe1 and IHe2) can not be rewritten as
+the dependent types of the stacks do not match.
+Thus for the dependent case we add n to the IH. 
+Otherwise this helper lemma is the same as rpn_eval1_applied
+*)
+Lemma rpn_eval2_applied :
+  forall (e : Exp) (f : env) (n:nat) (st : Vector.t lit n) (rpn : RPNvec (S n)),
+    rpn_eval2 (compiler2 e rpn) f st =
+    rpn_eval2 rpn f (eval e f :: st).
+Proof.
+  intros e f.
+  induction e;intros n.
+  (* Lit and Var case *)
+  - destruct n;reflexivity.
+  - destruct n;reflexivity.
+  (*Binop case*)
+  - intros st rpn. simpl.
+    rewrite IHe1.
+    rewrite IHe2. 
+    reflexivity.
+Qed.
+
+(*
+Prove that
+forall e:Exp, eval e = rpn_eval (rpn e)
+
+Aka: Prove equivalence with dependent types *)
+Lemma equivalent2 : forall (f:env) (e:Exp), 
+  eval e f = hd (rpn_eval2 (compiler2 e R_nil) f (nil lit)).
+Proof.
+  intros f e.
+  destruct e;
+  simpl;try reflexivity.
+  - rewrite rpn_eval2_applied.
+    rewrite rpn_eval2_applied.
+    reflexivity.
+Qed.
 
